ok

SStructTT/Defs/Syntax.lean
@@ -18,7 +18,7 @@ inductive Tm where
   | pair (m n : Tm) (r : Rlv) (s : Srt)
   | proj (A m n : Tm)
   | bool | tt | ff
-  | ifte (A m n1 n2 : Tm)
+  | ite (A m n1 n2 : Tm)
   | id   (A m n : Tm)
   | rfl  (m : Tm)
   | rw   (A h p : Tm)
@@ -44,7 +44,7 @@ def rename_rec (ξ : Var -> Var) (m : Tm Srt) : Tm Srt :=
   | bool => bool
   | tt => tt
   | ff => ff
-  | ifte A m n1 n2 => ifte (rename_rec (upren ξ) A) (rename_rec ξ m) (rename_rec ξ n1) (rename_rec ξ n2)
+  | ite A m n1 n2 => ite (rename_rec (upren ξ) A) (rename_rec ξ m) (rename_rec ξ n1) (rename_rec ξ n2)
   | id A m n => id (rename_rec ξ A) (rename_rec ξ m) (rename_rec ξ n)
   | rfl m => rfl (rename_rec ξ m)
   | rw A m n => rw (rename_rec (upren (upren ξ)) A) (rename_rec ξ m) (rename_rec ξ n)
@@ -66,7 +66,7 @@ variable (ξ : Var -> Var) (A B m n n1 n2 : Tm Srt) (x i : Nat) (r : Rlv) (s : S
 @[asimp]lemma bool : rename ξ (@bool Srt) = bool := by rfl
 @[asimp]lemma tt   : rename ξ (@tt Srt) = tt := by rfl
 @[asimp]lemma ff   : rename ξ (@ff Srt) = ff := by rfl
-@[asimp]lemma ifte : rename ξ (ifte A m n1 n2) = ifte (rename (upren ξ) A) (rename ξ m) (rename ξ n1) (rename ξ n2) := by rfl
+@[asimp]lemma ite : rename ξ (ite A m n1 n2) = ite (rename (upren ξ) A) (rename ξ m) (rename ξ n1) (rename ξ n2) := by rfl
 @[asimp]lemma id   : rename ξ (id A m n) = id (rename ξ A) (rename ξ m) (rename ξ n) := by rfl
 @[asimp]lemma rfl  : rename ξ (rfl m) = rfl (rename ξ m) := by rfl
 @[asimp]lemma rw   : rename ξ (rw A m n) = rw (rename (upren $ upren ξ) A) (rename ξ m) (rename ξ n) := by rfl
@@ -81,14 +81,14 @@ def subst_rec (σ : Var -> Tm Srt) (m : Tm Srt) : Tm Srt :=
   | app m n => app (subst_rec σ m) (subst_rec σ n)
   | sig A B r s => sig (subst_rec σ A) (subst_rec (up σ) B) r s
   | pair m n r s => pair (subst_rec σ m) (subst_rec σ n) r s
-  | proj A m n => proj (subst_rec (up σ) A) (subst_rec σ m) (subst_rec (up $ up σ) n)
+  | proj A m n => proj (subst_rec (up σ) A) (subst_rec σ m) (subst_rec (upn 2 σ) n)
   | bool => bool
   | tt => tt
   | ff => ff
-  | ifte A m n1 n2 => ifte (subst_rec (up σ) A) (subst_rec σ m) (subst_rec σ n1) (subst_rec σ n2)
+  | ite A m n1 n2 => ite (subst_rec (up σ) A) (subst_rec σ m) (subst_rec σ n1) (subst_rec σ n2)
   | id A m n => id (subst_rec σ A) (subst_rec σ m) (subst_rec σ n)
   | rfl m => rfl (subst_rec σ m)
-  | rw A m n => rw (subst_rec (up $ up σ) A) (subst_rec σ m) (subst_rec σ n)
+  | rw A m n => rw (subst_rec (upn 2 σ) A) (subst_rec σ m) (subst_rec σ n)
 
 instance : Subst (Tm Srt) where
   subst := subst_rec
@@ -103,14 +103,14 @@ variable (σ : Var -> Tm Srt) (A B m n n1 n2 : Tm Srt) (x i : Nat) (r : Rlv) (s 
 @[asimp]lemma app  : subst σ (app m n) = app (subst σ m) (subst σ n) := by rfl
 @[asimp]lemma sig  : subst σ (sig A B r s) = sig (subst σ A) (subst (up σ) B) r s := by rfl
 @[asimp]lemma pair : subst σ (pair m n r s) = pair (subst σ m) (subst σ n) r s := by rfl
-@[asimp]lemma proj : subst σ (proj A m n) = proj (subst (up σ) A) (subst σ m) (subst (up $ up σ) n) := by rfl
+@[asimp]lemma proj : subst σ (proj A m n) = proj (subst (up σ) A) (subst σ m) (subst (upn 2 σ) n) := by rfl
 @[asimp]lemma bool : subst σ (@bool Srt) = bool := by rfl
 @[asimp]lemma tt   : subst σ (@tt Srt) = tt := by rfl
 @[asimp]lemma ff   : subst σ (@ff Srt) = ff := by rfl
-@[asimp]lemma ifte : subst σ (ifte A m n1 n2) = ifte (subst (up σ) A) (subst σ m) (subst σ n1) (subst σ n2) := by rfl
+@[asimp]lemma ite : subst σ (ite A m n1 n2) = ite (subst (up σ) A) (subst σ m) (subst σ n1) (subst σ n2) := by rfl
 @[asimp]lemma id   : subst σ (id A m n) = id (subst σ A) (subst σ m) (subst σ n) := by rfl
 @[asimp]lemma rfl  : subst σ (rfl m) = rfl (subst σ m) := by rfl
-@[asimp]lemma rw   : subst σ (rw A m n) = rw (subst (up $ up σ) A) (subst σ m) (subst σ n) := by rfl
+@[asimp]lemma rw   : subst σ (rw A m n) = rw (subst (upn 2 σ) A) (subst σ m) (subst σ n) := by rfl
 end Subst
 
 section SubstLemmas
@@ -131,7 +131,7 @@ lemma rename_subst ξ (m : Tm Srt) : rename ξ m = m.[ren ξ] := by
   | bool => asimp
   | tt => asimp
   | ff => asimp
-  | ifte A m n1 n2 ihA ihm ihn1 ihn2 => asimp[up_upren, ihA, ihm, ihn1, ihn2]
+  | ite A m n1 n2 ihA ihm ihn1 ihn2 => asimp[up_upren, ihA, ihm, ihn1, ihn2]
   | id A m n ihA ihm ihn => asimp[ihA, ihm, ihn]
   | rfl m ihm => asimp[ihm]
   | rw A m n ihA ihm ihn => asimp[up_upren, ihA, ihm, ihn]
@@ -155,7 +155,7 @@ lemma subst_id (m : Tm Srt) : m.[ids] = m := by
   | bool => asimp
   | tt => asimp
   | ff => asimp
-  | ifte A m n1 n2 ihA ihm ihn1 ihn2 => asimp[up_ids, ihA, ihm, ihn1, ihn2]
+  | ite A m n1 n2 ihA ihm ihn1 ihn2 => asimp[up_ids, ihA, ihm, ihn1, ihn2]
   | id A m n ihA ihm ihn => asimp[ihA, ihm, ihn]
   | rfl m ihm => asimp[ihm]
   | rw A m n ihA ihm ihn => asimp[up_ids, ihA, ihm, ihn]
@@ -180,7 +180,7 @@ lemma ren_subst_comp ξ σ (m : Tm Srt) : m.[ren ξ].[σ] = m.[ξ !>> σ] := by
   | bool => asimp
   | tt => asimp
   | ff => asimp
-  | ifte A m n1 n2 ihA ihm ihn1 ihn2 => asimp[up_upren, up_comp_upren, ihA, ihm, ihn1, ihn2]
+  | ite A m n1 n2 ihA ihm ihn1 ihn2 => asimp[up_upren, up_comp_upren, ihA, ihm, ihn1, ihn2]
   | id A m n ihA ihm ihn => asimp[ihA, ihm, ihn]
   | rfl m ihm => asimp[ihm]
   | rw A m n ihA ihm ihn => asimp[up_upren, up_comp_upren, ihA, ihm, ihn]
@@ -209,7 +209,7 @@ lemma subst_ren_comp σ ξ (m : Tm Srt) : m.[σ].[ren ξ] = m.[σ !>> rename ξ]
   | bool => asimp
   | tt => asimp
   | ff => asimp
-  | ifte A m n1 n2 ihA ihm ihn1 ihn2 => asimp[up_upren, up_comp_ren, ihA, ihm, ihn1, ihn2]
+  | ite A m n1 n2 ihA ihm ihn1 ihn2 => asimp[up_upren, up_comp_ren, ihA, ihm, ihn1, ihn2]
   | id A m n ihA ihm ihn => asimp[ihA, ihm, ihn]
   | rfl m ihm => asimp[ihm]
   | rw A m n ihA ihm ihn => asimp[up_upren, up_comp_ren, ihA, ihm, ihn]
@@ -240,7 +240,7 @@ lemma subst_comp (σ τ : Var -> Tm Srt) m : m.[σ].[τ] = m.[σ >> τ] := by
   | bool => asimp
   | tt => asimp
   | ff => asimp
-  | ifte A m n1 n2 ihA ihm ihn1 ihn2 => asimp[up_comp, ihA, ihm, ihn1, ihn2]
+  | ite A m n1 n2 ihA ihm ihn1 ihn2 => asimp[up_comp, ihA, ihm, ihn1, ihn2]
   | id A m n ihA ihm ihn => asimp[ihA, ihm, ihn]
   | rfl m ihm => asimp[ihm]
   | rw A m n ihA ihm ihn => asimp[up_comp, ihA, ihm, ihn]
